\begin{Lemma}
	\label{tds:lemma_disj_acc_ch:lemma}
	Consider a Turing dynamical system with fundamental values $\Omega_1$ and $\Omega_2$.
	If the TDS has disjoint accepting chains, then \IM{\Omega_1 = \Omega_2}.
\end{Lemma}

\proof
	We have 
	\begin{align*}
		T^{-i}(\mathcal{F}_2) \cap \mathcal{F}_1 \subseteq \mathcal{F}_1 ~\text{for every}~ i \in \N_0
	\end{align*}
	and for $x \in \mathcal{F}_1$
	\begin{align*}
		T^i(x) \in \mathcal{F}_2 ~\text{for some}~ i \in \N_0
	\end{align*}
	and therefore
	\begin{align*}
		\mathcal{F}_1 = \bigcup_{i = 0}^\infty (T^{-i}(\mathcal{F}_2) \cap \mathcal{F}_1)
	\end{align*}
	However on $T^{-i}(\mathcal{F}_2)$ we have $T^\infty = T^i$. Because of disjoint accepting chains, $T^\infty$ and therefore also $T^i$ is injective on $\mathcal{F}_2$ except for some null-set.
	But then Lemma \ref{tds:lemma_tx_measurable:lemma} yields
	\begin{align*}
		\mu(T^i(T^{-i}(\mathcal{F}_2) \cap \mathcal{F}_1)) = \mu(T^{-i}(\mathcal{F}_2) \cap \mathcal{F}_1)
	\end{align*}
	Therefore
	\begin{align*}
		  &\Omega_1 \\
		=~&\mu(\mathcal{F}_1) \\
		=~&\mu(\bigcup_{i=0}^\infty T^{-i}(\mathcal{F}_2) \cap \mathcal{F}_1)) \\
		\leq~&\sum_{i=0}^\infty \mu(T^{-i}(\mathcal{F}_2) \cap \mathcal{F}_1) \\
		=~&\sum_{i=0}^\infty \mu(T^i(T^{-i}(\mathcal{F}_2) \cap \mathcal{F}_1)) \\
		\leq~&\sum_{i=0}^\infty \mu(\mathcal{F}_2 \cap T^i(\mathcal{F}_1)) \\
		=~&\mu(\bigcup_{i=0}^\infty \mathcal{F}_2 \cap T^i(\mathcal{F}_1)) \\
		=~&\mu(\mathcal{F}_2 \cap \bigcup_{i=0}^\infty T^i(\mathcal{F}_1)) \\
		=~&\mu(\mathcal{F}_2) \\
		=~&\Omega_2
	\end{align*}
	But again by Lemma \ref{tds:lemma_tx_measurable:lemma}, $T$ is measure contracting, so in particular we have \IM{\Omega_1 \geq \Omega_2} which proves equality.
\endproof